% Inductive Semantics.hoare

\newcommand{\cA}[1]{\textcolor{grey}{#1}}
\newcommand{\cB}[1]{\textcolor{red}{#1}}
\newcommand{\cC}[1]{\textcolor{blue}{#1}}

\begin{mathpar}
\inferrule* [Right=HNewObj]
{
    {\Gamma} \vdash {{x}} : {{C}}\\{\fields({C})} = {{\overline{f}}}}
{{\Gamma} \hoare {\hat{\phi}} {{{x} := \new {C}}} {\wo {\hat{\phi}} {x} \hsc {{({{x}} \neq {{\vnull}})} \hsc {\overline{\acc({x}, f_i)}}}}}
\end{mathpar}

\begin{mathpar}
\inferrule* [Right=HFieldAssign]
{{\wo {\hat{\phi}} {\acc(x.f)}} = \hat{\phi'}\\
    \hat{\phi} \implies {{\acc({{x}}.{f})}}\\{\Gamma} \vdash {{x}} : {{C}}\\{\Gamma} \vdash {{y}} : {T}\\\vdash {C}.{f} : {T}}
{{\Gamma} \hoare {\hat{\phi}} {{{x}.{f} := {y}}} {\hat{\phi'} \hsc {{\acc({{x}}.{f})} \hsc {{({{x}} \neq {{\vnull}})} \hsc {{({{{x}}.{f}} = {{y}})}}}}}}
\end{mathpar}

\begin{mathpar}
\inferrule* [Right=HVarAssign]
{{\wo {\hat{\phi}} {x}} = \hat{\phi'}\\
    {x} \not \in {FV({e})}\\{\Gamma} \vdash {{x}} : {T}\\{\Gamma} \vdash {e} : {T}\\{\hat{\phi'}} \implies {\accFor {{e}}}}
{{\Gamma} \hoare {\hat{\phi}} {{{x} := {e}}} {\hat{\phi'} \hsc {{({{x}} = {e})}}}}
\end{mathpar}

Have $\hsc$ take care of necessary congruent rewriting of $e$ in order to preserve self-framing!

\begin{mathpar}
\inferrule* [Right=HReturn]
{{\wo {\hat{\phi}} {\xresult}} = \hat{\phi'}\\
    {\Gamma} \vdash {{x}} : {T}\\{\Gamma} \vdash {{\xresult}} : {T}}
{{\Gamma} \hoare {\hat{\phi}} {{\return {x}}} {\hat{\phi'} \hsc {{({{\xresult}} = {{x}})}}}}
\end{mathpar}

\begin{mathpar}
\inferrule* [Right=HApp]
{\wo {\wo {\hat{\phi}} {x}} {\staticFP{\hat{\phi_p}}} = \hat{\phi'}\\
    {\Gamma} \vdash {{y}} : {{C}}\\{\mmethod({C}, {m})} = {{{T_r}~{m}({T_p}~{z})~{\requires \hat{\phi_{pre}};~\ensures \hat{\phi_{post}};}~\{ {\_} \}}}\\{\Gamma} \vdash {{x}} : {T_r}\\{\Gamma} \vdash {{z'}} : {T_p}\\\hat{\phi} \implies {{\hat{\phi_p}} \hsc {({{y}} \neq {{\vnull}})}}\\x \neq y \wedge x \neq z'\\\hat{\phi_p} = {\hat{\phi_{pre}}[{y}, {z'} / {\xthis}, {{z}}]}\\\hat{\phi_q} = {\hat{\phi_{post}}[{y}, {z'}, {x} / {\xthis}, {{z}}, {\xresult}]}}
{{\Gamma} \hoare {\hat{\phi}} {{{x} := {y}.{m}({z'})}} {\hat{\phi'} \hsc \hat{\phi_q}}}
\end{mathpar}

\begin{mathpar}
\inferrule* [Right=HAssertIrregular (grad lifting not piecewise)]
{\hat{\phi} \implies {\phi_a}}
{{\Gamma} \hoare {\hat{\phi}} {{\assert {\phi_a}}} {\hat{\phi}}}
\end{mathpar}

\begin{mathpar}
    \inferrule* [Right=HAssertBadIdea]
    {{\wo {\hat{\phi}} {\staticFP{\phi_a}}} = \hat{\phi'}\\
        \hat{\phi} \implies {\phi_a}}
    {{\Gamma} \hoare {\hat{\phi}} {{\assert {\phi_a}}} {\hat{\phi'} \hsc \phi_a}}
\end{mathpar}

\begin{mathpar}
	\inferrule* [Right=HAssert]
	{\imp(\phi_a)(\hat{\phi}) = \hat{\phi'}}
	{{\Gamma} \hoare {\hat{\phi}} {{\assert {\phi_a}}} {\hat{\phi'}}}
\end{mathpar}

\begin{mathpar}
\inferrule* [Right=HRelease]
{\imp(\phi_r)(\hat{\phi}) = \hat{\phi'}\\
{\wo {\hat{\phi'}} {\staticFP{\phi_r}}} = \hat{\phi''}}
{{\Gamma} \hoare {\hat{\phi}} {{\release {\phi_r}}} {\hat{\phi''}}}
\end{mathpar}

\begin{mathpar}
\inferrule* [Right=HDeclare]
{{x} \not\in \dom({\Gamma})\\{{\Gamma}, {x} : {T}} \hoare {\hat{\phi} \hsc {({{x}} = {{\texttt{defaultValue}({T})}})}} {\overline{s}} {\hat{\phi'}}}
{{\Gamma} \hoare {\hat{\phi}} {{{T}~{x}}; {\overline{s}}} {\hat{\phi'}}}
\end{mathpar}

\begin{mathpar}
\inferrule* [Right=HHold]
{
    \sfrmphi {\phi} \\
\imp(\phi)(\hat{\phi_f}) = \hat{\phi_f'}\\
\wo {\hat{\phi_f'}} {\staticFP{\phi}} = \hat{\phi_r}\\
\wo {\wo {\hat{\phi_f'}} {\staticFP{\hat{\phi_r}}}}{FV(\hat{\phi_f'}) \backslash FV(\hat{\phi})} = \hat{\phi'}\\
{\Gamma} \hoare {\hat{\phi_r}} {\overline{s}} {\hat {\phi_r'}}
}
{{\Gamma} \hoare {\hat{\phi_f}} {{\sHold {$\phi$} {${\overline{s}}$}}} {\phiCons{$\hat{\phi_r'}$}{$\hat{\phi'}$}}}
\end{mathpar}

\begin{mathpar}
\inferrule* [Right=HSec]
{{\Gamma} \hoare {\hat{\phi_p}} {s_1} {\hat{\phi_q}}\\{\Gamma} \hoare {\hat{\phi_q}} {\overline{s_2}} {\hat{\phi_r}}}
{{\Gamma} \hoare {\hat{\phi_p}} {{s_1}; \overline{s_2}} {\hat{\phi_r}}}
\end{mathpar}

